src/wacket.v
@@ -1,28 +1,53 @@
 Require Import Bool List ZArith.
+Require Import String.
 
-
+Local Open Scope Z_scope.
 
 (* based on the dupe language 
 https://www.cs.umd.edu/class/spring2022/cmsc430/Dupe.html *)
 
+Inductive dupeUniaryOp : Type :=
+| D_U_add1 
+| D_U_sub1 
+| D_U_zero
+.
+
+Definition uniOpToString (u :dupeUniaryOp) : string := match u with 
+| D_U_add1 => "add1"
+| D_U_sub1 => "sub1"
+| D_U_zero => "zero?"
+end.
+
 Inductive dupe: Type :=
 | D_Integer: Z -> dupe
 | D_Boolean: bool -> dupe
-| D_add1: dupe -> dupe
-| D_sub1: dupe -> dupe
-| D_zero: dupe -> dupe
+| D_UniOp: dupeUniaryOp -> dupe -> dupe
 | D_if: dupe -> dupe -> dupe -> dupe
 .
 
 Notation "#t" := true.
 Notation "#f" := false.
 
+Notation " 'add1' " := D_U_add1.
+Notation " 'sub1' " := D_U_sub1.
+Notation " 'zero?' " := D_U_zero.
+
 Notation "'(' 'Int' z ')'" := (D_Integer z).
 Notation "'(' 'Bool' b ')'" := (D_Boolean b).
-Notation "'(' 'add1' e ')'" := (D_add1 e).
-Notation "'(' 'sub1' e ')'" := (D_sub1 e).
-Notation "'(' 'zero?' e ')'" := (D_zero e).
+Notation "'(' 'Prim1' op exp ')'" := (D_UniOp op exp).
 Notation "'(' 'If' b 'Then' t 'Else' e ')'" := (D_if b t e).
+
+Inductive typ: Type :=
+| typ_Int
+| typ_Bool
+| typ_Error
+.
+
+Definition typeToString (t:typ) : string := match t with 
+| typ_Int => "Int"
+| typ_Bool => "Bool"
+| typ_Error => "Error"
+end.
 
 Inductive dupeResult : Type :=
 | DR_Int: Z -> dupeResult
@@ -30,25 +55,36 @@ Inductive dupeResult : Type :=
 | DR_Error: dupeResult
 .
 
+Definition resultType result := match result with 
+| DR_Int _ => typ_Int
+| DR_Bool _ => typ_Bool
+| DR_Error => typ_Error
+end.
+
+Definition uniOpExpectedType op := match op with 
+| D_U_add1 => typ_Int
+| D_U_sub1 => typ_Int
+| D_U_zero => typ_Int
+end. 
+
+Definition uniOpResultType op := match op with 
+| D_U_add1 => typ_Int
+| D_U_sub1 => typ_Int
+| D_U_zero => typ_Bool
+end. 
+
+Definition UniOpTransform op result := match (op, result) with 
+| (D_U_add1, DR_Int z) => DR_Int (z + 1)
+| (D_U_sub1, DR_Int z) => DR_Int (z - 1)
+| (D_U_zero, DR_Int z) => DR_Bool (z =? 0)
+| _ => DR_Error
+end.
+
 Fixpoint evalDupe(d : dupe) := match d with 
-| (Int z) => (DR_Int z)
-| (Bool b) => (DR_Bool b)
-| (add1 e) => match (evalDupe e) with 
-    | DR_Int i => DR_Int (i + 1)
-    | DR_Bool b => DR_Error
-    | DR_Error => DR_Error
-    end
-| (sub1 e) => match (evalDupe e) with 
-    | DR_Int i => DR_Int (i - 1)
-    | DR_Bool b => DR_Error
-    | DR_Error => DR_Error
-    end
-| (zero? e) => match (evalDupe e) with 
-    | DR_Int i => DR_Bool (Z.eqb i 0)
-    | DR_Bool b => DR_Error
-    | DR_Error => DR_Error
-    end
-| (If e1 Then e2 Else e3) => match (evalDupe e1) with 
+| (D_Integer z) => (DR_Int z)
+| (D_Boolean b) => (DR_Bool b)
+| D_UniOp op exp => UniOpTransform op (evalDupe exp)
+| (D_if e1 e2 e3) => match (evalDupe e1) with 
     | DR_Int i => evalDupe e2
     | DR_Bool b => if b then evalDupe e2  else evalDupe e3 
     | DR_Error => DR_Error
@@ -62,16 +98,10 @@ Inductive dupeEval: dupe -> dupeResult -> Prop :=
 | E_D_Interger: forall z, (D_Integer z) d==> (DR_Int z)
 | E_D_Boolean: forall b, (D_Boolean b) d==> (DR_Bool b)
 
-| E_D_add1: forall t z, 
-    t d==> (DR_Int z) ->
-    (D_add1 t) d==> (DR_Int (z + 1))
-| E_D_sub1: forall t z, 
-    t d==> (DR_Int z) ->
-    (D_sub1 t) d==> (DR_Int (z - 1))
-
-| E_D_isZero: forall t z,
-    t d==> (DR_Int z) ->
-    (D_zero t) d==> (DR_Bool (Z.eqb z 0))
+| E_D_UniOp: forall t v op,
+    t d==> v ->
+    (resultType v) = (uniOpExpectedType op) ->
+    (D_UniOp op t) d==> (UniOpTransform op v)
 
 | E_D_ifFalse: forall t_if t_then t_else v,
     t_if d==> (DR_Bool false) -> 
